checks/Examples.v
@@ -1,29 +1,88 @@
 Require Import List.
-Require Import String.
 
 Require Import Absyn.
 Require Import Env.
 Require Import Symbol.
+Require Import Types.
 
-Local Open Scope string.
+Module Type EX.
+  Parameter ex : Absyn.exp.
+End EX.
 
-Definition syms := Symbol.make_syms
-  ("a" :: "b" :: "c" :: "x" :: "y" :: "z" :: nil).
+Module AbsynListNotations.
+  Notation "D[ ]" := DNil.
+  Notation "D[ x ]" := (DCons x DNil).
+  Notation "D[ x ; .. ; y ]" := (DCons x .. (DCons y DNil) ..).
 
-Definition a := Symbol.symbol' "a" syms.
-Definition b := Symbol.symbol' "b" syms.
-Definition c := Symbol.symbol' "c" syms.
-Definition x := Symbol.symbol' "x" syms.
-Definition y := Symbol.symbol' "y" syms.
-Definition z := Symbol.symbol' "z" syms.
+  Notation "E[ ]" := ENil.
+  Notation "E[ x ]" := (ECons x ENil).
+  Notation "E[ x ; .. ; y ]" := (ECons x .. (ECons y ENil) ..).
+End AbsynListNotations.
 
-Definition int := Symbol.symbol' "int" Env.tsyms.
-Definition string := Symbol.symbol' "string" Env.tsyms.
+Import ListNotations.
+Import AbsynListNotations.
 
-Section VALID.
+Definition sy n := Symbol.symbol' n Symbol.sym_empty.
 
-End VALID.
+Module EX1 <: EX.
+  (* let
+       type arrtype = array of int
+       var arr1 : arrtype := arrtype [10] of 0
+     in
+       arr1
+     end *)
+  Definition s_arrtype := sy 20.
+  Definition s_arr1 := sy 21.
 
-Section INVALID.
+  Definition ex : exp :=
+    LetExp
+      D[TypeDec [mk_tydec s_arrtype (ArrayTy Env.s_int)];
+        VarDec (mk_vardec s_arr1 true) (Some s_arrtype) (ArrayExp s_arrtype (IntExp 10) (IntExp 0))]
+      (SeqExp
+        E[VarExp (SimpleVar s_arr1)]).
+End EX1.
 
-End INVALID.
+Module EX2 <: EX.
+  (* let
+       type myint = int
+       type arrtype = array of myint
+       var arr1 : arrtype := arrtype [10] of 0
+     in
+       arr1
+     end *)
+  Definition s_arrtype := sy 20.
+  Definition s_arr1 := sy 21.
+  Definition s_myint := sy 22.
+
+  Definition ex : exp :=
+    LetExp
+      D[TypeDec [mk_tydec s_myint (NameTy Env.s_int);
+                 mk_tydec s_arrtype (ArrayTy s_myint)];
+        VarDec (mk_vardec s_arr1 true) (Some s_arrtype) (ArrayExp s_arrtype (IntExp 10) (IntExp 0))]
+      (SeqExp
+        E[VarExp (SimpleVar s_arr1)]).
+End EX2.
+
+Module EX3 <: EX.
+  (* let
+       type rectype = {name : string, age : int}
+       var rec1 : rectype := rectype {name="Nobody", age=1000}
+     in
+       rec1.name := "Somebody";
+       rec1
+     end *)
+  Definition s_rectype := sy 20.
+  Definition s_name := sy 21.
+  Definition s_rec1 := sy 22.
+  Definition s_age := sy 23.
+
+  Definition ex : exp :=
+    LetExp
+      D[TypeDec [mk_tydec s_rectype (RecordTy [mk_tfield s_name Env.s_string;
+                                               mk_tfield s_age Env.s_int])];
+        VarDec (mk_vardec s_rec1 true) (Some s_rectype) (RecordExp E[StringExp "Nobody"; IntExp 1000]
+                                                                   [s_name; s_age] s_rectype)]
+      (SeqExp
+        E[AssignExp (FieldVar (SimpleVar s_rec1) s_name) (StringExp "Someboy");
+          VarExp (SimpleVar s_rec1)]).
+End EX3.
