checks/SemantChecks.v
@@ -1,11 +1,26 @@
 Require Import Absyn.
+Require Import Errors.
 Require Import Examples.
 Require Import Semant.
 Require Import Types.
 
 Section TypeDec_CHECKS.
 
-  Definition td_check (td : dec) :=
-    exists ce us, wt_dec base_cenv Types.uinit td ce us.
+  Definition checkEx (ex : Absyn.exp) :=
+    exists ty us, transProg ex = OK (ty, us).
+
+  Ltac solve := 
+    match goal with
+    | [ |- checkEx ?E ] => unfold checkEx; unfold E; unfold transProg; simpl; eauto
+    end.
+
+  Example ex1 : checkEx EX1.ex.
+  Proof. solve. Qed.
+
+  Example ex2 : checkEx EX2.ex.
+  Proof. solve. Qed.
+
+  Example ex3 : checkEx EX3.ex.
+  Proof. solve. Qed.
 
 End TypeDec_CHECKS.
