Env.v
@@ -1,5 +1,4 @@
 Require Import List.
-Require Import String.
 
 Require Import Symbol.
 Require Import Types.
@@ -39,26 +38,37 @@ Module Env <: ENV.
     Symbol.enter tbl (Symbol.symbol' (fst entry) stbl) (snd entry).
 
   Definition tsyms : Symbol.sym_tbl := Symbol.make_syms
-    ("int" :: "string" :: nil)%string.
+    (0 :: 1 :: nil).
+  Definition s_int := Symbol.symbol' 0 tsyms.
+  Definition s_string := Symbol.symbol' 1 tsyms.
 
   Definition vsyms : Symbol.sym_tbl := Symbol.make_syms
-    ("print" :: "flush" :: "getchar" :: "ord" :: "chr" :: "size" :: "substring"
-     :: "concat" :: "not" :: "exit" :: nil)%string.
+    (0 :: 1 :: 2 :: 3 :: 4 :: 5 :: 6 :: 7 :: 8 :: 9 :: nil).
+  Definition s_print := Symbol.symbol' 0 vsyms.
+  Definition s_flush := Symbol.symbol' 1 vsyms.
+  Definition s_getchar := Symbol.symbol' 2 vsyms.
+  Definition s_ord := Symbol.symbol' 3 vsyms.
+  Definition s_chr := Symbol.symbol' 4 vsyms.
+  Definition s_size := Symbol.symbol' 5 vsyms.
+  Definition s_substring := Symbol.symbol' 6 vsyms.
+  Definition s_concat := Symbol.symbol' 7 vsyms.
+  Definition s_not := Symbol.symbol' 8 vsyms.
+  Definition s_exit := Symbol.symbol' 9 vsyms.
 
   Definition base_tenv := fold_right (enter tsyms) Symbol.empty
-    (("int", Types.INT) :: ("string", Types.STRING) :: nil)%string.
+    ((s_int, Types.INT) :: (s_string, Types.STRING) :: nil).
 
   Definition base_venv := fold_right (enter vsyms) Symbol.empty
-    (("print", FunEntry (Types.STRING :: nil) Types.UNIT)
-     :: ("flush", FunEntry nil Types.UNIT)
-     :: ("getchar", FunEntry nil Types.STRING)
-     :: ("ord", FunEntry (Types.STRING :: nil) Types.INT)
-     :: ("chr", FunEntry (Types.INT :: nil) Types.STRING)
-     :: ("size", FunEntry (Types.STRING :: nil) Types.INT)
-     :: ("substring", FunEntry (Types.STRING :: Types.INT :: Types.INT :: nil) Types.STRING)
-     :: ("concat", FunEntry (Types.STRING :: Types.STRING :: nil) Types.STRING)
-     :: ("not", FunEntry (Types.INT :: nil) Types.INT)
-     :: ("exit", FunEntry (Types.INT :: nil) Types.UNIT)
-     :: nil)%string.
+    ((s_print, FunEntry (Types.STRING :: nil) Types.UNIT)
+     :: (s_flush, FunEntry nil Types.UNIT)
+     :: (s_getchar, FunEntry nil Types.STRING)
+     :: (s_ord, FunEntry (Types.STRING :: nil) Types.INT)
+     :: (s_chr, FunEntry (Types.INT :: nil) Types.STRING)
+     :: (s_size, FunEntry (Types.STRING :: nil) Types.INT)
+     :: (s_substring, FunEntry (Types.STRING :: Types.INT :: Types.INT :: nil) Types.STRING)
+     :: (s_concat, FunEntry (Types.STRING :: Types.STRING :: nil) Types.STRING)
+     :: (s_not, FunEntry (Types.INT :: nil) Types.INT)
+     :: (s_exit, FunEntry (Types.INT :: nil) Types.UNIT)
+     :: nil).
 
 End Env.
